rules/rules_integer.v
@@ -1,0 +1,119 @@
+(*
+
+  Copyright 2014 Cornell University
+  Copyright 2015 Cornell University
+  Copyright 2016 Cornell University
+  Copyright 2017 Cornell University
+
+  This file is part of VPrl (the Verified Nuprl project).
+
+  VPrl is free software: you can redistribute it and/or modify
+  it under the terms of the GNU General Public License as published by
+  the Free Software Foundation, either version 3 of the License, or
+  (at your option) any later version.
+
+  VPrl is distributed in the hope that it will be useful,
+  but WITHOUT ANY WARRANTY; without even the implied warranty of
+  MERCHANTABILITY or FITNESS FOR A PARTICULAR PURPOSE.  See the
+  GNU General Public License for more details.
+
+  You should have received a copy of the GNU General Public License
+  along with VPrl.  If not, see <http://www.gnu.org/licenses/>.
+
+
+  Websites: http://nuprl.org/html/verification/
+            http://nuprl.org/html/Nuprl2Coq
+            https://github.com/vrahli/NuprlInCoq
+
+  Authors: Abhishek Anand & Vincent Rahli
+
+*)
+
+
+Require Export sequents2.
+Require Export sequents_lib.
+Require Export rules_useful.
+Require Export subst_tacs_aeq.
+Require Export cequiv_tacs.
+Require Export per_props_equality.
+Require Export sequents_equality.
+
+
+
+(**
+
+<<
+   H |- n in Z
+
+     By integer_equality(n)
+>>
+ *)
+
+Definition rule_integer_equality_concl {o} (H : @bhyps o) (n : Z) :=
+  mk_baresequent H (mk_conclax (mk_member (mk_integer n) mk_int)).
+
+Definition rule_integer_equality {o}
+             (H : @barehypotheses o)
+             (n : Z) :=
+  mk_rule
+    (rule_integer_equality_concl H n)
+    [ ]
+    [ ].
+
+Lemma rule_integer_equality_true3 {o} :
+  forall lib
+         (H : @barehypotheses o)
+         (n : Z),
+    rule_true3 lib (rule_integer_equality H n).
+Proof.
+  intros.
+  unfold rule_integer_equality, rule_true3, wf_bseq, closed_type_baresequent, closed_extract_baresequent; simpl.
+  intros.
+  repnd.
+  clear cargs hyps.
+
+  (* We prove the well-formedness of things *)
+  destseq; allsimpl.
+
+  assert (wf_csequent (rule_integer_equality_concl H n)) as wfc.
+  { unfold wf_csequent, wf_sequent, wf_concl; simpl.
+    allrw @vswf_hypotheses_nil_eq.
+    dands; auto.
+    apply covered_axiom. }
+  exists wfc.
+  unfold wf_csequent, wf_sequent, wf_concl in wfc; repnd; allsimpl; proof_irr; GC.
+
+  vr_seq_true.
+  lsubst_tac.
+  rw @tequality_mkc_member_sp.
+  rw @equality_in_member.
+  dands; auto;
+    try (apply tequality_int);
+    try (complete (right; spcast; auto));
+    try (complete (spcast; apply computes_to_valc_refl; eauto 2 with slow));
+    try (complete (apply equality_in_int; exists n; dands;
+                   spcast; apply computes_to_valc_refl; eauto 2 with slow)).
+Qed.
+
+Lemma rule_integer_equality_true_ext_lib {o} :
+  forall lib
+         (H : @barehypotheses o)
+         (n : Z),
+    rule_true_ext_lib lib (rule_integer_equality H n).
+Proof.
+  introv.
+  apply rule_true3_implies_rule_true_ext_lib.
+  introv.
+  apply rule_integer_equality_true3.
+Qed.
+
+Lemma rule_integer_equality_true {o} :
+  forall lib
+         (H : @barehypotheses o)
+         (n : Z),
+    rule_true lib (rule_integer_equality H n).
+Proof.
+  introv.
+  apply rule_true3_implies_rule_true.
+  apply rule_integer_equality_true3.
+Qed.
